Distribute run_codegen over bind; delete dlist

theories/compiler/codegen.v
@@ -3,28 +3,26 @@ Import ListNotations.
 Require Import Coq.Program.Basics.
 Local Open Scope program_scope.
 
+Require Import stdpp.base.
+
+From ExtLib.Data Require Import List.
 From ExtLib.Data.Monads Require Import StateMonad WriterMonad.
-From ExtLib.Structures Require Import Monads.
-Import MonadNotation.
-Local Open Scope monad.
+From ExtLib.Structures Require Import Monoid Monads.
 
 From Wasm Require datatypes.
 
-From RichWasm Require term.
+Require RichWasm.term.
 From RichWasm.compiler Require Import types util.
-Require Import RichWasm.util.dlist.
-Import RichWasm.util.dlist.Notation.
+Require Import RichWasm.util.stdpp_extlib.
 
 Module R := RichWasm.term.
 Module W := Wasm.datatypes.
 
 Notation wlocal_ctx := (list W.value_type) (only parsing).
 
-Notation dexpr := (dlist W.basic_instruction).
-
 Record codegen (A : Type) :=
   { uncodegen : stateT wlocal_ctx
-                       (writerT (@DList.Monoid_dlist W.basic_instruction)
+                       (writerT (@Monoid_list_app W.basic_instruction)
                                 (sum error))
                        A }.
 
@@ -35,7 +33,7 @@ Existing Instance Monad_stateT.
 
 Global Instance Monad_codegen : Monad codegen :=
   { ret := fun _ => Build_codegen ∘ ret;
-    bind := fun _ _ c f => Build_codegen (uncodegen c >>= uncodegen ∘ f) }.
+    bind := fun _ _ c f => Build_codegen (uncodegen c ≫= uncodegen ∘ f) }.
 
 Global Instance MonadExc_codegen : MonadExc error codegen :=
   { raise := fun _ => Build_codegen ∘ raise;
@@ -45,13 +43,13 @@ Global Instance MonadState_codegen : MonadState wlocal_ctx codegen :=
   { get := Build_codegen get;
     put := Build_codegen ∘ put }.
 
-Global Instance MonadWriter_codegen : MonadWriter (@DList.Monoid_dlist W.basic_instruction) codegen :=
+Global Instance MonadWriter_codegen : MonadWriter (@Monoid_list_app W.basic_instruction) codegen :=
   { tell := Build_codegen ∘ tell;
     listen := fun _ => Build_codegen ∘ listen ∘ uncodegen;
     (* Work around broken implementation of `pass` in ExtLib.
        https://github.com/rocq-community/coq-ext-lib/issues/153 *)
     pass := fun _ c => Build_codegen (mkStateT (fun s =>
-      pass ('(x, f, s) <- runStateT (uncodegen c) s;;
+      pass ('(x, f, s) ← runStateT (uncodegen c) s;
             ret (x, s, f)))) }.
 
 Definition lift_error {A} (c : error + A) : codegen A :=
@@ -67,30 +65,155 @@ Definition ignore {A} (c : codegen A) : codegen unit :=
   c;;
   ret tt.
 
-Definition run_codegen (c : codegen unit) (wl : wlocal_ctx) : error + wlocal_ctx * W.expr :=
+Definition run_codegen {A} (c : codegen A) (wl : wlocal_ctx) : error + A * wlocal_ctx * W.expr :=
   match runWriterT (runStateT (uncodegen c) wl) with
   | inl e => inl e
-  | inr x => inr (snd (PPair.pfst x), DList.to_list (PPair.psnd x))
+  | inr x => inr (PPair.pfst x, PPair.psnd x)
   end.
 
 Definition emit (e : W.basic_instruction) : codegen unit :=
-  tell (DList.singleton e).
+  tell [e].
 
-Definition capture {A} (c : codegen A) : codegen (A * dexpr) :=
-  censor (const []%DL) (listen c).
+Definition capture {A} (c : codegen A) : codegen (A * W.expr) :=
+  censor (const []) (listen c).
 
 Definition block_c {A} (tf : W.function_type) (c : codegen A) : codegen A :=
-  '(x, es) <- capture c;;
-  emit (W.BI_block tf (DList.to_list es));;
+  '(x, es) ← capture c;
+  emit (W.BI_block tf es);;
   ret x.
 
 Definition loop_c {A} (tf : W.function_type) (c : codegen A) : codegen A :=
-  '(x, es) <- capture c;;
-  emit (W.BI_loop tf (DList.to_list es));;
+  '(x, es) ← capture c;
+  emit (W.BI_loop tf es);;
   ret x.
 
 Definition if_c {A B} (tf : W.function_type) (thn : codegen A) (els : codegen B) : codegen (A * B) :=
-  '(x1, es1) <- capture thn;;
-  '(x2, es2) <- capture els;;
-  emit (W.BI_if tf (DList.to_list es1) (DList.to_list es2));;
+  '(x1, es1) ← capture thn;
+  '(x2, es2) ← capture els;
+  emit (W.BI_if tf es1 es2);;
   ret (x1, x2).
+
+Lemma runWriterT_sum_bind_dist {A B L E}
+  (m : Monoid L)
+  (c : writerT m (sum E) A)
+  (f : A -> writerT m (sum E) B)
+  (x : B)
+  (l l1 : L) :
+  runWriterT (c ≫= f) = inr (PPair.ppair x l) ->
+  exists x1 l1 l2,
+  runWriterT c = inr (PPair.ppair x1 l1) /\
+  runWriterT (f x1) = inr (PPair.ppair x l2) /\
+  l = m.(monoid_plus) l1 l2.
+Proof.
+  intros H.
+  unfold runWriterT, mbind, stdpp_extlib.MBind_Monad, flip, bind, Monad_writerT, bind, EitherMonad.Monad_either in H.
+  destruct c.
+  cbn in H.
+  destruct runWriterT; first congruence.
+  exists (PPair.pfst p).
+  exists (PPair.psnd p).
+  destruct (f (PPair.pfst p)).
+  cbn in H.
+  destruct runWriterT; first congruence.
+  cbn.
+  exists (PPair.psnd p0).
+  split; first reflexivity.
+  split.
+  - inversion H. reflexivity.
+  - congruence.
+Qed.
+
+Lemma runState_bind_dist {A B S} (c : state S A) (f : A -> state S B) s s' x :
+  runState (c ≫= f) s = (x, s') <->
+  exists x1 s1,
+  runState c s = (x1, s1) /\
+  runState (f x1) s1 = (x, s').
+Proof.
+  split.
+  {
+    intros H.
+    unfold mbind, stdpp_extlib.MBind_Monad, flip, bind, Monad_state, runState in H.
+    unfold runState.
+    destruct c.
+    destruct (runState s).
+    exists a, s0.
+    split; first reflexivity.
+    assumption.
+  }
+  {
+    intros (x1 & s1 & H1 & H2).
+    unfold mbind, stdpp_extlib.MBind_Monad, flip, bind, Monad_state.
+    cbn.
+    rewrite H1.
+    assumption.
+  }
+Qed.
+
+Lemma runWriterT_runStateT_sum_bind_dist {E L S A B}
+  (m : Monoid L)
+  (c : stateT S (writerT m (sum E)) A)
+  (f : A -> stateT S (writerT m (sum E)) B)
+  (s s' : S)
+  (l : L)
+  (x : B) :
+  runWriterT (runStateT (c ≫= f) s) = inr (PPair.ppair (x, s') l) ->
+  exists x1 s1 l1 l2,
+  runWriterT (runStateT c s) = inr (PPair.ppair (x1, s1) l1) /\
+  runWriterT (runStateT (f x1) s1) = inr (PPair.ppair (x, s') l2) /\
+  l = m.(monoid_plus) l1 l2.
+Proof.
+  intros H.
+  unfold mbind, stdpp_extlib.MBind_Monad, runStateT, flip, bind, Monad_stateT in H.
+  apply runWriterT_sum_bind_dist in H.
+  destruct H as (x1 & l1 & l2 & H1 & H2 & H3).
+  - destruct x1 as [x1 s1].
+    exists x1.
+    exists s1.
+    exists l1.
+    exists l2.
+    split; first assumption.
+    split; assumption.
+  - apply l.
+Qed.
+
+Lemma run_codegen_def {A} (c : codegen A) wl wl' x es:
+  run_codegen c wl = inr (x, wl', es) <->
+  runWriterT (runStateT (uncodegen c) wl) = inr (PPair.ppair (x, wl') es).
+Proof.
+  split.
+  {
+    intros H.
+    unfold run_codegen in H.
+    destruct (runWriterT (runStateT (uncodegen c) wl)); first congruence.
+    inversion H.
+    reflexivity.
+  }
+  {
+    intros H.
+    unfold run_codegen.
+    destruct (runWriterT (runStateT (uncodegen c) wl)); first congruence.
+    inversion H.
+    reflexivity.
+  }
+Qed.
+
+Lemma run_codegen_bind_dist {A B} (c : codegen A) (f : A -> codegen B) wl wl' es x :
+  run_codegen (c ≫= f) wl = inr (x, wl', es) ->
+  exists x1 wl1 es1 es2,
+  run_codegen c wl = inr (x1, wl1, es1) /\
+  run_codegen (f x1) wl1 = inr (x, wl', es2) /\
+  es = es1 ++ es2.
+Proof.
+  intros H.
+  rewrite run_codegen_def in H.
+  apply runWriterT_runStateT_sum_bind_dist in H.
+  destruct H as (x1 & s1 & l1 & l2 & H1 & H2 & H3).
+  exists x1, s1, l1, l2.
+  rewrite !run_codegen_def.
+  split.
+  - assumption.
+  - split.
+    + assumption.
+    + unfold monoid_plus, Monoid_list_app in H3.
+      assumption.
+Qed.
